Progress on reasoning about GOL runs

gol_rulesScript.sml
@@ -102,4 +102,165 @@ Definition to_state_def:
   to_state xs = { p | MEM (p,T) xs } : state
 End
 
+(* runs *)
+
+Datatype:
+  modifier =
+    <| area           : (int # int) set ;
+       deletions      : (int # int) set ;
+       insertions     : (int # int) set ;
+       assert_area    : (int # int) set ;
+       assert_content : (int # int) set |>
+End
+
+Definition mod_step_def:
+  mod_step c s1 s3 ⇔
+    ∃s2.
+      infl s1 ⊆ c.area ∧
+      step s1 = s2 ∧
+      s2 ∩ c.assert_area = c.assert_content ∧
+      s3 = c.insertions ∪ (s2 DIFF c.deletions)
+End
+
+Theorem mod_step_univ:
+  c.area = UNIV ∧ c.insertions = EMPTY ∧ c.deletions = EMPTY
+  ⇒
+  (mod_step c s1 s2
+   ⇔
+   step s1 = s2 ∧
+   s2 ∩ c.assert_area = c.assert_content)
+Proof
+  gvs [mod_step_def] \\ metis_tac []
+QED
+
+Definition mod_steps_def:
+  mod_steps 0 c n s1 s2 = (s1 = s2) ∧
+  mod_steps (SUC k) c n s1 s3 =
+     ∃s2. mod_step (c n) s1 s2 ∧ mod_steps k c (n+1:num) s2 s3
+End
+
+Definition run_to_def:
+  run_to k c s t ⇔ mod_steps k c 0 s t
+End
+
+Definition run_def:
+  run c s = ∀k. ∃t. run_to k c s t
+End
+
+Definition disjoint_mod_def:
+  disjoint_mod m1 m2 ⇔ DISJOINT m1.area m2.area
+End
+
+Definition disjoint_mods_def:
+  disjoint_mods c1 c2 ⇔ ∀n. disjoint_mod (c1 n) (c2 n)
+End
+
+Definition mod_wf_def:
+  mod_wf m ⇔
+    m.deletions ⊆ m.area ∧
+    m.assert_area ⊆ m.area ∧
+    m.assert_content ⊆ m.assert_area
+End
+
+Definition mods_wf_def:
+  mods_wf c = ∀n. mod_wf (c (n:num))
+End
+
+Definition join_def:
+  join c1 c2  =
+    λn. <| area           := (c1 n).area ∪ (c2 n).area ;
+           deletions      := (c1 n).deletions ∪ (c2 n).deletions ;
+           insertions     := (c1 n).insertions ∪ (c2 n).insertions ;
+           assert_area    := (c1 n).assert_area ∪ (c2 n).assert_area ;
+           assert_content := (c1 n).assert_content ∪ (c2 n).assert_content |>
+End
+
+Theorem mod_steps_compose:
+  ∀c1 c2 k n s1 s2 t1 t2.
+    disjoint_mods c1 c2 ∧
+    mods_wf c1 ∧
+    mods_wf c2 ∧
+    mod_steps k c1 n s1 t1 ∧
+    mod_steps k c2 n s2 t2 ⇒
+    mod_steps k (join c1 c2) n (s1 ∪ s2) (t1 ∪ t2)
+Proof
+  gen_tac \\ gen_tac \\ Induct \\ gvs [mod_steps_def]
+  \\ rpt strip_tac \\ gvs []
+  \\ last_x_assum drule_all
+  \\ rename [‘_ (u1 ∪ u2) (_ ∪ _)’]
+  \\ disch_then $ irule_at Any
+  \\ gvs [mod_step_def,join_def]
+  \\ gvs [infl_union,mods_wf_def,disjoint_mods_def,disjoint_mod_def]
+  \\ rpt $ first_x_assum $ qspec_then ‘n’ assume_tac
+  \\ gvs [mod_wf_def]
+  \\ DEP_REWRITE_TAC [infl_compose]
+  \\ qabbrev_tac ‘u1 = step s1’
+  \\ qabbrev_tac ‘u2 = step s2’
+  \\ ‘u1 ⊆ infl s1’ by gvs [step_SUBSET_infl,Abbr‘u1’]
+  \\ ‘u2 ⊆ infl s2’ by gvs [step_SUBSET_infl,Abbr‘u2’]
+  \\ gvs [IN_DISJOINT,EXTENSION,SUBSET_DEF]
+  \\ metis_tac []
+QED
+
+(*
+  deletions and insertions --> assertions
+*)
+
+Definition can_assert_def:
+  can_assert p c ⇔
+    ∀n:num.
+      p ∩ (c n).deletions ≠ EMPTY ⇒
+      p ⊆ (c n).deletions ∧
+      p ⊆ (c n).assert_area ∧
+      (c n).insertions ∩ p = (c n).assert_content ∩ p
+End
+
+Definition assert_mod_def:
+  assert_mod p m =
+    if p ∩ m.deletions = EMPTY then m else
+      m with <| insertions := m.insertions DIFF p ;
+                deletions := m.deletions DIFF p |>
+End
+
+Definition assert_def:
+  assert p c = λn. assert_mod p (c n)
+End
+
+Theorem to_assert:
+  ∀k n s t.
+    mod_steps k c n s t ∧
+    can_assert p c
+    ⇒
+    mod_steps k (assert p c) n s t
+Proof
+  Induct
+  \\ gvs [mod_steps_def,PULL_EXISTS]
+  \\ rpt strip_tac \\ gvs []
+  \\ last_x_assum $ drule_then $ irule_at Any
+  \\ gvs [can_assert_def]
+  \\ first_x_assum $ qspec_then ‘n’ assume_tac
+  \\ gvs [mod_step_def,assert_def,assert_mod_def]
+  \\ IF_CASES_TAC \\ gvs []
+  \\ gvs [EXTENSION,SUBSET_DEF]
+  \\ metis_tac []
+QED
+
+
+
+
+
+(*
+params:
+ - inputs
+ - outputs
+ - asserts
+ - init state
+sets:
+ - area
+ - insertions
+ - deletions
+ - state s
+ - assertions
+*)
+
 val _ = export_theory();
